src/Pipit.Exp.Base.fst
@@ -1,17 +1,25 @@
 module Pipit.Exp.Base
 
 type prim2 =
-  | And | Or | Implies | Eq // | ...
+  | AndB | OrB | ImpliesB
+  | EqZ
+  | AddZ | SubZ | LeZ // | ...
 
-let value  = bool
+let value  = int
 let var    = nat
 
-let eval_prim2 (p: prim2) (v1 : value) (v2: value) =
+let bool_of_value (v: value): bool = v <> 0
+let value_of_bool (b: bool): value = if b then 1 else 0
+
+let eval_prim2 (p: prim2) (v1 : value) (v2: value): value =
   match p with
-  | And  -> v1 && v2
-  | Or   -> v1 || v2
-  | Implies -> if v1 then v2 else true
-  | Eq -> v1 = v2
+  | AndB  -> value_of_bool (bool_of_value v1 && bool_of_value v2)
+  | OrB   -> value_of_bool (bool_of_value v1 || bool_of_value v2)
+  | ImpliesB -> if bool_of_value v1 then v2 else 1
+  | EqZ -> value_of_bool (v1 = v2)
+  | AddZ -> v1 + v2
+  | SubZ -> v1 - v2
+  | LeZ -> value_of_bool (v1 <= v2)
 
 type exp =
   // v
@@ -20,6 +28,8 @@ type exp =
   | XVar   : var -> exp
   // f(e,...)
   | XPrim2 : prim2 -> exp -> exp -> exp
+  // if ep then et else ef
+  | XIte   : exp -> exp -> exp -> exp
   // pre e
   | XPre   : exp -> exp
   // e -> e'
@@ -29,13 +39,14 @@ type exp =
   // let x = e in e[x]
   | XLet   : exp -> exp -> exp
 
-let xpre_init: value = true
+let xpre_init: value = 0
 
 let rec wf (e: exp) (n: var): prop =
 match e with
 | XVal _ -> True
 | XVar x -> (x < n) == true
 | XPrim2 _ e1 e2 -> wf e1 n /\ wf e2 n
+| XIte ep et ef -> wf ep n /\ wf et n /\ wf ef n
 | XPre e1 -> wf e1 n
 | XThen e1 e2 -> wf e1 n /\ wf e2 n
 | XMu e1 -> wf e1 (n + 1)
@@ -49,6 +60,10 @@ let rec wf_weaken (e: exp) (n: var) (n': var { n <= n' }):
   | XVal _ -> ()
   | XVar x' -> ()
   | XPrim2 _ e1 e2 ->
+    wf_weaken e1 n n';
+    wf_weaken e2 n n'
+  | XIte ep e1 e2 ->
+    wf_weaken ep n n';
     wf_weaken e1 n n';
     wf_weaken e2 n n'
   | XPre e1 -> wf_weaken e1 n n'
