src/Pipit.System.Exp.fst
@@ -1,88 +1,89 @@
-(* Transition systems *)
+(* Shelved - translation to transition system with proof *)
 module Pipit.System.Exp
 
-open Pipit.System.Base
 
-open Pipit.Exp.Base
-open Pipit.Exp.Bigstep
-open Pipit.Exp.Causality
+// open Pipit.System.Base
 
-module C = Pipit.Context
+// open Pipit.Exp.Base
+// open Pipit.Exp.Bigstep
+// open Pipit.Exp.Causality
 
-(* A system we get from translating an expression *)
-let xsystem (input: nat) (state: Type) = system (C.row input) state value
+// module C = Pipit.Context
 
-let xsystem_stepn
-  (#outer #vars: nat)
-  (#state: Type)
-  (t: xsystem vars state)
-  (streams: C.table outer vars)
-  (vs: C.vector value outer)
-  (s': state): prop =
-  let C.Table rs = streams in
-  system_stepn t rs vs s'
+// (* A system we get from translating an expression *)
+// let xsystem (input: nat) (state: Type) = system (C.row input) state value
+
+// let xsystem_stepn
+//   (#outer #vars: nat)
+//   (#state: Type)
+//   (t: xsystem vars state)
+//   (streams: C.table outer vars)
+//   (vs: C.vector value outer)
+//   (s': state): prop =
+//   let C.Table rs = streams in
+//   system_stepn t rs vs s'
 
 
-let rec state_of_exp (e: exp): Type =
-  match e with
-  | XVal v -> unit
-  | XVar x -> unit
-  | XPrim2 p e1 e2 -> state_of_exp e1 * state_of_exp e2
-  | XPre e1 -> state_of_exp e1 * value
-  | XThen e1 e2 -> bool * state_of_exp e2
-  | XMu e1 -> state_of_exp e1
+// let rec state_of_exp (e: exp): Type =
+//   match e with
+//   | XVal v -> unit
+//   | XVar x -> unit
+//   | XPrim2 p e1 e2 -> state_of_exp e1 * state_of_exp e2
+//   | XPre e1 -> state_of_exp e1 * value
+//   | XThen e1 e2 -> bool * state_of_exp e2
+//   | XMu e1 -> state_of_exp e1
 
-let rec system_of_exp (e: exp) (vars: nat { wf e vars }):
-    xsystem vars (state_of_exp e) =
-  match e with
-  | XVal v -> system_const v
-  | XVar x -> system_map (fun i -> C.row_index i x) system_input
-  | XPrim2 p e1 e2 ->
-    system_map2 (eval_prim2 p) (system_of_exp e1 vars) (system_of_exp e2 vars)
-  | XPre e1 ->
-    system_pre xpre_init (system_of_exp e1 vars)
-  | XThen e1 e2 ->
-    system_then (system_of_exp e1 vars) (system_of_exp e2 vars)
-  | XMu e1 ->
-    let t = system_of_exp e1 (vars + 1) in
-    system_mu #(C.row vars) #(C.row (vars + 1)) (fun i v -> C.row_append (C.row1 v) i) t
+// let rec system_of_exp (e: exp) (vars: nat { wf e vars }):
+//     xsystem vars (state_of_exp e) =
+//   match e with
+//   | XVal v -> system_const v
+//   | XVar x -> system_map (fun i -> C.row_index i x) system_input
+//   | XPrim2 p e1 e2 ->
+//     system_map2 (eval_prim2 p) (system_of_exp e1 vars) (system_of_exp e2 vars)
+//   | XPre e1 ->
+//     system_pre xpre_init (system_of_exp e1 vars)
+//   | XThen e1 e2 ->
+//     system_then (system_of_exp e1 vars) (system_of_exp e2 vars)
+//   | XMu e1 ->
+//     let t = system_of_exp e1 (vars + 1) in
+//     system_mu #(C.row vars) #(C.row (vars + 1)) (fun i v -> C.row_append (C.row1 v) i) t
 
-let rec system_of_exp_invariant
-  (#outer #vars: nat)
-  (e: exp { wf e vars /\ causal e })
-  (streams: C.table outer vars)
-  (vs: C.vector value outer)
-  (hBS: bigstep streams e vs)
-  (s: state_of_exp e):
-    Tot prop (decreases e) =
-  match e with
-  | XVar _ -> unit
-  | XVal _ -> unit
-  | XPrim2 _ e1 e2 ->
-    let (s1, s2) = s <: (state_of_exp e1 * state_of_exp e2) in
-    let BSPrim2 _ _ _ _ vs1 vs2 hBS1 hBS2 = hBS in
-    system_of_exp_invariant e1 streams vs1 hBS1 s1 /\
-    system_of_exp_invariant e2 streams vs2 hBS2 s2
-  | XPre e1 ->
-    begin
-    match hBS with
-      | BSPre0 e -> True
-      | BSPre _ _ _ vs1 hBS1 ->
-    let v1'   = bigstep_monotone_inv_next #(outer - 1) #vars #streams hBS1 in
-    let hBS1' = bigstep_monotone_inv #(outer - 1) #vars #streams hBS1 in
-    let (s1, v1) = s <: (state_of_exp e1 * value) in
-    (system_of_exp_invariant #outer #vars e1 streams (v1' :: vs1) hBS1' s1 /\ v1 == v1')
-  end
+// let rec system_of_exp_invariant
+//   (#outer #vars: nat)
+//   (e: exp { wf e vars /\ causal e })
+//   (streams: C.table outer vars)
+//   (vs: C.vector value outer)
+//   (hBS: bigstep streams e vs)
+//   (s: state_of_exp e):
+//     Tot prop (decreases e) =
+//   match e with
+//   | XVar _ -> unit
+//   | XVal _ -> unit
+//   | XPrim2 _ e1 e2 ->
+//     let (s1, s2) = s <: (state_of_exp e1 * state_of_exp e2) in
+//     let BSPrim2 _ _ _ _ vs1 vs2 hBS1 hBS2 = hBS in
+//     system_of_exp_invariant e1 streams vs1 hBS1 s1 /\
+//     system_of_exp_invariant e2 streams vs2 hBS2 s2
+//   | XPre e1 ->
+//     begin
+//     match hBS with
+//       | BSPre0 e -> True
+//       | BSPre _ _ _ vs1 hBS1 ->
+//     let v1'   = bigstep_monotone_inv_next #(outer - 1) #vars #streams hBS1 in
+//     let hBS1' = bigstep_monotone_inv #(outer - 1) #vars #streams hBS1 in
+//     let (s1, v1) = s <: (state_of_exp e1 * value) in
+//     (system_of_exp_invariant #outer #vars e1 streams (v1' :: vs1) hBS1' s1 /\ v1 == v1')
+//   end
 
-  | XThen e1 e2 ->
-    let (init, s2) = coerce_eq #_ #(bool * state_of_exp e2) () s in
-    let BSThen _ _ _ vs1 vs2 hBS1 hBS2 = hBS in
-    (init = (outer > 0)) /\ system_of_exp_invariant e2 streams vs2 hBS2 s2
-  | XMu e1 ->
-    let s1 = coerce_eq #_ #(state_of_exp e1) () s in
-    let BSMu _ _ vs1 hBS1 = hBS in
-    let hBS' = bigstep_substitute_XMu e1 streams vs hBS in
-    system_of_exp_invariant #outer #(vars + 1) e1 (C.table_map_append (C.table_of_values vs1) streams) vs1 hBS' s1
+//   | XThen e1 e2 ->
+//     let (init, s2) = coerce_eq #_ #(bool * state_of_exp e2) () s in
+//     let BSThen _ _ _ vs1 vs2 hBS1 hBS2 = hBS in
+//     (init = (outer > 0)) /\ system_of_exp_invariant e2 streams vs2 hBS2 s2
+//   | XMu e1 ->
+//     let s1 = coerce_eq #_ #(state_of_exp e1) () s in
+//     let BSMu _ _ vs1 hBS1 = hBS in
+//     let hBS' = bigstep_substitute_XMu e1 streams vs hBS in
+//     system_of_exp_invariant #outer #(vars + 1) e1 (C.table_map_append (C.table_of_values vs1) streams) vs1 hBS' s1
 
 // TODO temp disable proof while simplifying transform
 // let rec step0_ok
@@ -198,14 +199,14 @@ let rec system_of_exp_invariant
 //     Lemma (exists (s': state_of_exp e). xsystem_stepn #(outer - 1) #vars (system_of_exp e vars) streams vs s') =
 //   let (| s', () |) = step_many_ok e streams vs hBS in ()
 
-let system_eval_complete
-  (#outer: nat) (#vars: nat)
-  (e: exp { causal e /\ wf e vars })
-  (streams: C.table outer vars)
-  (vs: C.vector value outer)
-  (hBS: bigstep streams e vs):
-    Lemma (exists (s': state_of_exp e). xsystem_stepn #outer #vars (system_of_exp e vars) streams vs s') =
-  admit ()
+// let system_eval_complete
+//   (#outer: nat) (#vars: nat)
+//   (e: exp { causal e /\ wf e vars })
+//   (streams: C.table outer vars)
+//   (vs: C.vector value outer)
+//   (hBS: bigstep streams e vs):
+//     Lemma (exists (s': state_of_exp e). xsystem_stepn #outer #vars (system_of_exp e vars) streams vs s') =
+//   admit ()
 
 // let system_eval_complete'
 //   (#outer: nat) (#vars: nat)
