src/Pipit.System.Ind.fst
@@ -1,3 +1,4 @@
+(* Inductive proofs on transition systems *)
 module Pipit.System.Ind
 
 open Pipit.System.Base
@@ -9,14 +10,14 @@ let rec prop_for_all (l: list prop): prop =
  | [] -> True
  | p :: ps -> p /\ prop_for_all ps
 
-let base_case' (#input #state: Type) (t: system input state bool): prop =
-  forall (i: input) (s: state) (s': state) (r: bool).
-    t.init s ==> t.step i s s' r ==> r
+let base_case' (#input #state: Type) (t: system input state C.value): prop =
+  forall (i: input) (s: state) (s': state) (r: C.value).
+    t.init s ==> t.step i s s' r ==> r <> 0
 
-let step_case' (#input #state: Type) (t: system input state bool): prop =
-  forall (i0 i1: input) (s0: state) (s1 s2: state) (r0 r1: bool).
-    t.step i0 s0 s1 r0 ==> r0 ==>
-    t.step i1 s1 s2 r1 ==> r1
+let step_case' (#input #state: Type) (t: system input state C.value): prop =
+  forall (i0 i1: input) (s0: state) (s1 s2: state) (r0 r1: C.value).
+    t.step i0 s0 s1 r0 ==> r0 <> 0 ==>
+    t.step i1 s1 s2 r1 ==> r1 <> 0
 
 let base_case (#input #state: Type) (t: system input state prop): prop =
   forall (i: input) (s: state) (s': state) (r: prop).
@@ -51,12 +52,12 @@ let rec induct1_sound (#len: nat) (#input #state: Type)
    with h.
      induct1_sound #(len - 1) t (i0 :: is) (p0 :: ps) s1
 
-let bmc2' (#input #state: Type) (t: system input state bool): prop =
-  forall (i1 i2: input) (s0 s1 s2: state) (r1 r2: bool).
+let bmc2' (#input #state: Type) (t: system input state C.value): prop =
+  forall (i1 i2: input) (s0 s1 s2: state) (r1 r2: C.value).
     t.init s0 ==>
     t.step i1 s0 s1 r1 ==>
     t.step i2 s1 s2 r2 ==>
-    r2
+    r2 <> 0
 
 let bmc2 (#input #state: Type) (t: system input state prop): prop =
   forall (i1 i2: input) (s0 s1 s2: state) (r1 r2: prop).
@@ -65,43 +66,44 @@ let bmc2 (#input #state: Type) (t: system input state prop): prop =
     t.step i2 s1 s2 r2 ==>
     r2
 
-open Pipit.Exp.Base
-open Pipit.Exp.Bigstep
-open Pipit.Exp.Causality
+(* Shelved: proof that properties proved for transition systems apply to original expression *)
+// open Pipit.Exp.Base
+// open Pipit.Exp.Bigstep
+// open Pipit.Exp.Causality
 
-open Pipit.System.Exp
+// open Pipit.System.Exp
 
-let exp_valid (e: exp) (vars: nat) = wf e vars /\ causal e
+// let exp_valid (e: exp) (vars: nat) = wf e vars /\ causal e
 
-let exp_for_all (e: exp) (vars: nat): prop =
-  forall (len: nat)
-    (inputs: C.table len vars)
-    (vs: C.vector value len)
-    (hBS: bigstep inputs e vs).
-    List.Tot.for_all (fun r -> r) vs
+// let exp_for_all (e: exp) (vars: nat): prop =
+//   forall (len: nat)
+//     (inputs: C.table len vars)
+//     (vs: C.vector value len)
+//     (hBS: bigstep inputs e vs).
+//     List.Tot.for_all (fun r -> r <> 0) vs
 
-let prop_of_bool (b: bool): prop = b == true
+// let prop_of_value (v: value): prop = ~ (v = 0)
 
-let rec prop_for_all__prop_of_bool (bs: list bool):
-  Lemma (requires prop_for_all (C.vector_map #(List.Tot.length bs) prop_of_bool bs))
-        (ensures List.Tot.for_all (fun r -> r) bs) =
- // TODO prop_for_all__prop_of_bool easy
- admit ()
+// let rec prop_for_all__prop_of_bool (vs: list value):
+//   Lemma (requires prop_for_all (C.vector_map #(List.Tot.length vs) prop_of_value vs))
+//         (ensures List.Tot.for_all (fun r -> r <> 0) vs) =
+//  // TODO prop_for_all__prop_of_bool easy
+//  admit ()
 
-let induct1_exp (#vars: nat)
-  (e: exp { exp_valid e vars }):
-  Lemma (requires induct1 (system_map prop_of_bool (system_of_exp e vars)))
-        (ensures exp_for_all e vars) =
-  introduce forall (len: nat) (inputs: C.vector (C.row vars) len) (vs: C.vector bool len) (hBS: bigstep (C.Table inputs) e vs). List.Tot.for_all (fun r -> r) vs
-  with
-  begin
-    system_eval_complete e (C.Table inputs) vs hBS;
-    eliminate exists (s': (state_of_exp e)). system_stepn (system_of_exp e vars) inputs vs s'
-    returns _
-    with hEx.
-    begin
-        system_map_sem prop_of_bool (system_of_exp e vars) inputs vs s';
-        induct1_sound (system_map prop_of_bool (system_of_exp e vars)) inputs (C.vector_map prop_of_bool vs) s';
-        prop_for_all__prop_of_bool vs
-    end
-  end
+// let induct1_exp (#vars: nat)
+//   (e: exp { exp_valid e vars }):
+//   Lemma (requires induct1 (system_map prop_of_value (system_of_exp e vars)))
+//         (ensures exp_for_all e vars) =
+//   introduce forall (len: nat) (inputs: C.vector (C.row vars) len) (vs: C.vector bool len) (hBS: bigstep (C.Table inputs) e vs). List.Tot.for_all (fun r -> r) vs
+//   with
+//   begin
+//     system_eval_complete e (C.Table inputs) vs hBS;
+//     eliminate exists (s': (state_of_exp e)). system_stepn (system_of_exp e vars) inputs vs s'
+//     returns _
+//     with hEx.
+//     begin
+//         system_map_sem prop_of_bool (system_of_exp e vars) inputs vs s';
+//         induct1_sound (system_map prop_of_bool (system_of_exp e vars)) inputs (C.vector_map prop_of_bool vs) s';
+//         prop_for_all__prop_of_bool vs
+//     end
+//   end
