src/Pipit.Sugar.fst
@@ -1,0 +1,63 @@
+(* Meagre syntactic sugar for constructing expressions.
+  Want a HOAS-to-de-bruijn transform. *)
+module Pipit.Sugar
+
+open Pipit.Exp.Base
+
+(* Literals *)
+let tt = XVal 1
+let ff = XVal 0
+
+let z (i: int) = XVal i
+let z0 = z 0
+let z1 = z 1
+
+(* Variable helpers *)
+let x0 = XVar 0
+let x1 = XVar 1
+let x2 = XVar 2
+
+(* Working with booleans *)
+let (/\) = XPrim2 AndB
+let (\/) = XPrim2 OrB
+let (=>) = XPrim2 ImpliesB
+
+(* Arithmetic operators, "^" suffix means "lifted" but unfortunately boolean operators such as /\^ do not parse *)
+let (=^) = XPrim2 EqZ
+let (+^) = XPrim2 AddZ
+let (-^) = XPrim2 SubZ
+let (<=^)  = XPrim2 LeZ
+
+let (!) (e1: exp) = e1 =^ ff
+
+let negate (e1: exp) = z0 -^ e1
+
+(* if-then-else *)
+let ite (ep et ef: exp) = XIte ep et ef
+
+(* unitialised delay *)
+let pre (e: exp) = XPre e
+
+(* "p -> q" in Lustre, first element of p followed by remainder of q *)
+let (-->) (e1 e2: exp) = XThen e1 e2
+
+(* unsafe binding forms / variable management *)
+let mu' (e: exp): exp = XMu e
+let let' (e1 e2: exp): exp = XLet e1 e2
+let lift' (e: exp) = Pipit.Exp.Subst.lift e 0
+
+(* modal logic operators: G (always in the past) *)
+let sofar (e: exp): exp =
+  mu' (lift' e /\ (tt --> pre x0))
+
+(* F (at least once in the past) *)
+let once (e: exp): exp =
+  mu' (lift' e \/ (ff --> pre x0))
+
+(* count of consecutively true *)
+let countsecutive (e: exp): exp =
+  mu' (ite (lift' e) (pre x0 +^ z1) z0)
+
+(* last-n, true for last n ticks *)
+let last (n: nat) (e: exp): exp =
+  z n <=^ countsecutive e
